FokkerChallenge/BLC/Blc.lean
@@ -13,10 +13,9 @@ def main : IO Unit := do
   let terms := terms.filter (fun t => !Cslib.LambdaCalculus.LocallyNameless.Untyped.Term.argOk t)
   let terms := terms.filter (fun t => !Cslib.LambdaCalculus.LocallyNameless.Untyped.Term.properClosedNoParens t)
 
-  let terms := terms.filter (fun t => Cslib.LambdaCalculus.LocallyNameless.Untyped.Term.size t >= 7)
   let terms := terms.filter (fun t => t ∉ Cslib.LambdaCalculus.LocallyNameless.Untyped.Term.fokkerUndecidedTerms)
+  let terms := terms.filter (fun t => t ∉ Cslib.LambdaCalculus.LocallyNameless.Untyped.Term.fokkerUpdatedOpenCerts.map Prod.fst)
 
-  let terms := terms.filter (fun t => !Cslib.LambdaCalculus.LocallyNameless.Untyped.Term.has_beta_redex t)
 
   let len := terms.length
   IO.println s!"{len} undecided"
